<?xml version="1.0"?>

<!DOCTYPE rdf:RDF [
    <!ENTITY rn "https://github.com/EmrahGuder/Renarration/#" >
	<!ENTITY oa "http://www.w3.org/ns/oa#" >
    <!ENTITY dcterms "http://purl.org/dc/terms/" >
    <!ENTITY foaf "http://xmlns.com/foaf/0.1/" >
    <!ENTITY dctypes "http://purl.org/dc/dcmitype/" >
    <!ENTITY owl "http://www.w3.org/2002/07/owl#" >
    <!ENTITY cnt "http://www.w3.org/2011/content#" >
    <!ENTITY dc "http://purl.org/dc/elements/1.1/" >
    <!ENTITY xsd "http://www.w3.org/2001/XMLSchema#" >
    <!ENTITY skos "http://www.w3.org/2004/02/skos/core#" >
    <!ENTITY rdfs "http://www.w3.org/2000/01/rdf-schema#" >
    <!ENTITY rdf "http://www.w3.org/1999/02/22-rdf-syntax-ns#" >
]>

<rdf:RDF xmlns="https://github.com/EmrahGuder/Renarration/"
     xml:base="https://github.com/EmrahGuder/Renarration/"
     xmlns:dc="http://purl.org/dc/elements/1.1/"
     xmlns:foaf="http://xmlns.com/foaf/0.1/"
     xmlns:cnt="http://www.w3.org/2011/content#"
     xmlns:dcterms="http://purl.org/dc/terms/"
     xmlns:rdfs="http://www.w3.org/2000/01/rdf-schema#"
     xmlns:oa="http://www.w3.org/ns/oa#"
     xmlns:xsd="http://www.w3.org/2001/XMLSchema#"
     xmlns:owl="http://www.w3.org/2002/07/owl#"
     xmlns:rdf="http://www.w3.org/1999/02/22-rdf-syntax-ns#"
     xmlns:dctypes="http://purl.org/dc/dcmitype/"
     xmlns:skos="http://www.w3.org/2004/02/skos/core#">
	 
    <owl:Ontology rdf:about="https://github.com/EmrahGuder/Renarration/#">
        <dcterms:modified rdf:datatype="&xsd;dateTime">2015-12-05T15:50:23+03:00</dcterms:modified>
        <owl:versionInfo>20151205_1</owl:versionInfo>
        <dc:title xml:lang="en">Renarration Data Model</dc:title>
        <dc:creator xml:lang="en">Emrah Guder</dc:creator>
        <dc:creator xml:lang="it">Suzan Uskudarli</dc:creator>
        <dc:contributor xml:lang="en">T. B. Dinesh</dc:contributor>
        <rdfs:comment xml:lang="en">
			Renarration Data Model specifies a framework for creating alternative narrations of source documents by 
			transformation of their elements such as translation of a paragraph or replacing an element with an image. 
		
			The specification can be found on GitHub - https://github.com/EmrahGuder/Renarration.			
		</rdfs:comment>
        <dc:description xml:lang="en">
			Renarration Data Model specifies a framework for creating alternative narrations of source documents by 
			transformation of their elements such as translation of a paragraph or replacing an element with an image. 
			
			A Renarration is considered to be an alternative narration described by a given user at a given time consisting 
			of a set of renarration transformations. The following figure shows renarration of a source document. 
			The source document is renarrated by a set of transformations on the elements of the document, as a result target document is composed. 
			The whole process is called a Renarration.
			
        </dc:description>
    </owl:Ontology>	 
	
	<!-- Data Properties -->
	
	<owl:DatatypeProperty rdf:about="&rn;renarratedAt">
        <rdfs:label xml:lang="en">renarratedAt</rdfs:label>
        <rdfs:comment xml:lang="en">
			The time at which the Renarration is created. There must be exactly one rn:renarratedAt property associated with a Renarration.
		</rdfs:comment>
        <rdfs:range rdf:resource="&xsd;dateTimeStamp"/>
        <rdfs:isDefinedBy rdf:resource="https://github.com/EmrahGuder/Renarration/#"/>
        <rdfs:domain rdf:resource="&rn;Renarration"/>
    </owl:DatatypeProperty>
	
	<owl:DatatypeProperty rdf:about="&rn;createdAt">
        <rdfs:label xml:lang="en">createdAt</rdfs:label>
        <rdfs:comment xml:lang="en">
			The time at which the Renarration Transformation is created. There must be exactly one rn:createdAt property associated with a Renarration Transformation.
		</rdfs:comment>
        <rdfs:range rdf:resource="&xsd;dateTimeStamp"/>
        <rdfs:isDefinedBy rdf:resource="https://github.com/EmrahGuder/Renarration/#"/>
        <rdfs:domain rdf:resource="&rn;RenarrationTransformation"/>
    </owl:DatatypeProperty>		
	
	<owl:DatatypeProperty rdf:about="&rn;prefix">
        <rdfs:label xml:lang="en">prefix</rdfs:label>
        <rdfs:comment xml:lang="en">
			The snippet of text occurs before the targeted text in a resource.
		</rdfs:comment>
        <rdfs:isDefinedBy rdf:resource="https://github.com/EmrahGuder/Renarration/#"/>
        <rdfs:domain rdf:resource="&rn;PrefixSuffixSelector"/>
    </owl:DatatypeProperty>	

	<owl:DatatypeProperty rdf:about="&rn;suffix">
        <rdfs:label xml:lang="en">suffix</rdfs:label>
        <rdfs:comment xml:lang="en">
			The snippet of text occurs after the targeted text in a resource.
		</rdfs:comment>
        <rdfs:isDefinedBy rdf:resource="https://github.com/EmrahGuder/Renarration/#"/>
        <rdfs:domain rdf:resource="&rn;PrefixSuffixSelector"/>
    </owl:DatatypeProperty>	
	
	<owl:DatatypeProperty rdf:about="&rn;selectedText">
        <rdfs:label xml:lang="en">selectedText</rdfs:label>
        <rdfs:comment xml:lang="en">
			The snippet of text which is selected.
		</rdfs:comment>
        <rdfs:isDefinedBy rdf:resource="https://github.com/EmrahGuder/Renarration/#"/>
        <rdfs:domain rdf:resource="&rn;PrefixSuffixSelector"/>
    </owl:DatatypeProperty>		
	
	<owl:DatatypeProperty rdf:about="&rn;offset">
        <rdfs:label xml:lang="en">offset</rdfs:label>
        <rdfs:comment xml:lang="en">
			The starting position of the content to be selected.
		</rdfs:comment>
        <rdfs:isDefinedBy rdf:resource="https://github.com/EmrahGuder/Renarration/#"/>
        <rdfs:domain rdf:resource="&rn;PrefixSuffixSelector"/>
		<rdfs:range rdf:resource="&xsd;nonNegativeInteger"/>
    </owl:DatatypeProperty>		
	
	<owl:DatatypeProperty rdf:about="&rn;byteNumber">
        <rdfs:label xml:lang="en">byteNumber</rdfs:label>
        <rdfs:comment xml:lang="en">
			The number of bytes should be selected after the value of rn:offset
		</rdfs:comment>
        <rdfs:isDefinedBy rdf:resource="https://github.com/EmrahGuder/Renarration/#"/>
        <rdfs:domain rdf:resource="&rn;PrefixSuffixSelector"/>
		<rdfs:range rdf:resource="&xsd;nonNegativeInteger"/>
    </owl:DatatypeProperty>		
	
	<!-- Data Properties -->
	
	<!-- Object Properties -->
	
    <owl:ObjectProperty rdf:about="&rn;renarratedBy">
        <rdfs:label xml:lang="en">renarratedBy</rdfs:label>
        <rdfs:comment xml:lang="en">
			The relationship between a Renarration and a Renarrator. There must be at least one rn:renarratedBy relationship associated with a Renarration. 
			The object of the relationship must be an instance of rn:Renarrator class, which is the person who is responsible for the creation of the Renarration.
		</rdfs:comment>
        <rdfs:isDefinedBy rdf:resource="https://github.com/EmrahGuder/Renarration/#"/>
        <rdfs:domain rdf:resource="&rn;Renarration"/>
		<rdfs:range rdf:resource="&rn;Renarrator"/>
    </owl:ObjectProperty>	
	
    <owl:ObjectProperty rdf:about="&rn;onSourceDocument">
        <rdfs:label xml:lang="en">onSourceDocument</rdfs:label>
        <rdfs:comment xml:lang="en">
			The relationship between a Renarration and a source document. There must be at least one rn:onSourceDocument relationship associated with a Renarration. 
			The object of the relationship must be a document for which the renarration is being done.
		</rdfs:comment>
        <rdfs:isDefinedBy rdf:resource="https://github.com/EmrahGuder/Renarration/#"/>
        <rdfs:domain rdf:resource="&rn;Renarration"/>
    </owl:ObjectProperty>	

    <owl:ObjectProperty rdf:about="&rn;toTargetDocument">
        <rdfs:label xml:lang="en">toTargetDocument</rdfs:label>
        <rdfs:comment xml:lang="en">
			The relationship between a Renarration and a source document. There must be at least one rn:onSourceDocument relationship associated with a Renarration. 
			The object of the relationship must be a document for which the renarration is being done.
		</rdfs:comment>
        <rdfs:isDefinedBy rdf:resource="https://github.com/EmrahGuder/Renarration/#"/>
        <rdfs:domain rdf:resource="&rn;Renarration"/>
    </owl:ObjectProperty>			
	
    <owl:ObjectProperty rdf:about="&rn;hasRenarrationTransformation">
        <rdfs:label xml:lang="en">hasRenarrationTransformation</rdfs:label>
        <rdfs:comment xml:lang="en">
			The relationship between a Renarration and a target document (renarrated document). 
			There must be at least one rn:toTargetDocument relationship associated with a Renarration. 
			The object of the relationship must be an instance of one or a list of renarration transform.
		</rdfs:comment>
        <rdfs:isDefinedBy rdf:resource="https://github.com/EmrahGuder/Renarration/#"/>
		<rdfs:domain rdf:resource="&rn;Renarration"/>
    </owl:ObjectProperty>	

    <owl:ObjectProperty rdf:about="&rn;hasNarration">
        <rdfs:label xml:lang="en">hasNarration</rdfs:label>
        <rdfs:comment xml:lang="en">
			The relationship between a Renarration Transformation and a narration defining content being created(as a renarration) for source content.
		</rdfs:comment>
        <rdfs:isDefinedBy rdf:resource="https://github.com/EmrahGuder/Renarration/#"/>
        <rdfs:domain rdf:resource="&rn;RenarrationTransformation"/>
    </owl:ObjectProperty>		
	
    <owl:ObjectProperty rdf:about="&rn;accessedFrom">
        <rdfs:label xml:lang="en">accessedFrom</rdfs:label>
        <rdfs:comment xml:lang="en">
			The relation between a narration and external resource from which the content may be referenced.
		</rdfs:comment>
        <rdfs:isDefinedBy rdf:resource="https://github.com/EmrahGuder/Renarration/#"/>
    </owl:ObjectProperty>	

    <owl:ObjectProperty rdf:about="&rn;sourceDocumentSelection">
        <rdfs:label xml:lang="en">sourceDocumentSelection</rdfs:label>
        <rdfs:comment xml:lang="en">
			The relationship between a Renarration Transformation and fragment of a source document. The object of the relationship must be an instance of a selector class.
		</rdfs:comment>
        <rdfs:isDefinedBy rdf:resource="https://github.com/EmrahGuder/Renarration/#"/>
		<rdfs:domain rdf:resource="&rn;RenarrationTransformation"/>
    </owl:ObjectProperty>		

    <owl:ObjectProperty rdf:about="&rn;targetDocumentSelection">
        <rdfs:label xml:lang="en">targetDocumentSelection</rdfs:label>
        <rdfs:comment xml:lang="en">
			The relationship between a Renarration Transformation and part of the renarrated document. The object of the relationship must be an instance of a selector class.
		</rdfs:comment>
        <rdfs:isDefinedBy rdf:resource="https://github.com/EmrahGuder/Renarration/#"/>
		<rdfs:domain rdf:resource="&rn;RenarrationTransformation"/>
    </owl:ObjectProperty>

    <owl:ObjectProperty rdf:about="&rn;actionOnDocument">
        <rdfs:label xml:lang="en">actionOnDocument</rdfs:label>
        <rdfs:comment xml:lang="en">
			The relationship between rn:RenarrationTransformation and rn:Action for defining type of action on targeted source element.
		</rdfs:comment>
        <rdfs:isDefinedBy rdf:resource="https://github.com/EmrahGuder/Renarration/#"/>
		<rdfs:domain rdf:resource="&rn;RenarrationTransformation"/>
		<rdfs:range rdf:resource="&rn;Action"/>
    </owl:ObjectProperty>	
	
    <owl:ObjectProperty rdf:about="&rn;sourceSelection">
        <rdfs:label xml:lang="en">sourceSelection</rdfs:label>
        <rdfs:comment xml:lang="en">
			The relationship between renarration transform and an instance of document selector for selecting part of a source document associated with the renarration.
		</rdfs:comment>
        <rdfs:isDefinedBy rdf:resource="https://github.com/EmrahGuder/Renarration/#"/>
		<rdfs:domain rdf:resource="&rn;RenarrationTransformation"/>
		<rdfs:range rdf:resource="&rn;DocumentSelector"/>
    </owl:ObjectProperty>	
	
    <owl:ObjectProperty rdf:about="&rn;targetSelection">
        <rdfs:label xml:lang="en">targetSelection</rdfs:label>
        <rdfs:comment xml:lang="en">
			The relationship between renarration transform and an instance of document selector for linking the selected part in renarrated document with source document.
		</rdfs:comment>
        <rdfs:isDefinedBy rdf:resource="https://github.com/EmrahGuder/Renarration/#"/>
		<rdfs:domain rdf:resource="&rn;RenarrationTransformation"/>
		<rdfs:range rdf:resource="&rn;DocumentSelector"/>
    </owl:ObjectProperty>			

    <owl:ObjectProperty rdf:about="&rn;isBetween">
        <rdfs:label xml:lang="en">isBetween</rdfs:label>
        <rdfs:comment xml:lang="en">
			The relation between a rn:BetweenSelector and rn:List. The object of the relationship must be an instance of rn:List class.
		</rdfs:comment>
        <rdfs:isDefinedBy rdf:resource="https://github.com/EmrahGuder/Renarration/#"/>
		<rdfs:domain rdf:resource="&rn;BetweenSelector"/>
		<rdfs:range rdf:resource="&rn;List"/>
    </owl:ObjectProperty>	

    <owl:ObjectProperty rdf:about="&rn;hasMotivation">
        <rdfs:label xml:lang="en">hasMotivation</rdfs:label>
        <rdfs:comment xml:lang="en">
			The relationship between a renarration and motivation.
		</rdfs:comment>
        <rdfs:isDefinedBy rdf:resource="https://github.com/EmrahGuder/Renarration/#"/>
		<rdfs:domain rdf:resource="&rn;Renarration"/>
		<rdfs:range rdf:resource="&rn;Motivation"/>
    </owl:ObjectProperty>	
	
    <owl:ObjectProperty rdf:about="&rn;hasTargetAudience">
        <rdfs:label xml:lang="en">hasTargetAudience</rdfs:label>
        <rdfs:comment xml:lang="en">
			The relationship between a renarration and a group of people renarration is aimed for.
		</rdfs:comment>
        <rdfs:isDefinedBy rdf:resource="https://github.com/EmrahGuder/Renarration/#"/>
		<rdfs:domain rdf:resource="&rn;Renarration"/>
    </owl:ObjectProperty>

    <owl:ObjectProperty rdf:about="&rn;nodes">
        <rdfs:label xml:lang="en">nodes</rdfs:label>
        <rdfs:comment xml:lang="en">
			The relationship between a resource and an instance of rdf:List class. When the relationship is rn:RenarrationTransformation 
			rn:nodes is used to define a list of Renarration Transformation. When the relationship is rn:hasNarration, it is used to define 
			a list of narrations(rn:hasNarration). Lastly, when the relationship is rn:onSourceDocument, it is used to define nested selections of source documents.
		</rdfs:comment>
        <rdfs:isDefinedBy rdf:resource="https://github.com/EmrahGuder/Renarration/#"/>
		<rdfs:domain rdf:resource="&rn;List"/>
		<rdfs:subPropertyOf rdf:resource="&rdfs;member"/>
    </owl:ObjectProperty>	
	
	<!-- Object Properties -->
	
	<!-- Classes -->
	
    <owl:Class rdf:about="&rn;Renarration">
        <rdfs:label xml:lang="en">Renarration</rdfs:label>
        <rdfs:comment xml:lang="en">
			The class for Renarrations. The rn:Renarration class must be associated with a renarrator(rn:Renarrator) and a timestamp for defining time at renarration is created.
		</rdfs:comment>
        <rdfs:isDefinedBy rdf:resource="https://github.com/EmrahGuder/Renarration/#"/>
    </owl:Class>	
	
    <owl:Class rdf:about="&rn;Renarrator">
        <rdfs:label xml:lang="en">Renarrator</rdfs:label>
        <rdfs:comment xml:lang="en">
			The class for Renarrators. Each renarrator must be equivalent with foaf:Person.
		</rdfs:comment>
        <rdfs:isDefinedBy rdf:resource="https://github.com/EmrahGuder/Renarration/#"/>
    </owl:Class>	

    <owl:Class rdf:about="&rn;Document">
        <rdfs:label xml:lang="en">Document</rdfs:label>
        <rdfs:comment xml:lang="en">
			Any type of resource on the Web. If a more specific type is known, than it should be associated with source or renarrated documents.
		</rdfs:comment>
        <rdfs:isDefinedBy rdf:resource="https://github.com/EmrahGuder/Renarration/#"/>
    </owl:Class>	
	
    <owl:Class rdf:about="&rn;RenarrationTransformation">
        <rdfs:label xml:lang="en">RenarrationTransformation</rdfs:label>
        <rdfs:comment xml:lang="en">
			The class for Renarration Transformations defining specific actions on parts of source documents. 
			The rn:RenarrationTransformation class must be associated with a Renarration, 
			a source document and a narration created for the selected part of the source document.
		</rdfs:comment>
        <rdfs:isDefinedBy rdf:resource="https://github.com/EmrahGuder/Renarration/#"/>
    </owl:Class>	
	
    <owl:Class rdf:about="&rn;Action">
        <rdfs:label xml:lang="en">Action</rdfs:label>
        <rdfs:comment xml:lang="en">
			The rn:Action class must be associated with a Renarration Transformation. Defines type of action on targeted source element.
		</rdfs:comment>
        <rdfs:isDefinedBy rdf:resource="https://github.com/EmrahGuder/Renarration/#"/>
		<rdfs:subClassOf rdf:resource="&skos;Concept"/>
    </owl:Class>

    <owl:Class rdf:about="&rn;DocumentSelector">
        <rdfs:label xml:lang="en">DocumentSelector</rdfs:label>
        <rdfs:comment xml:lang="en">
			The superclass for all selectors.
		</rdfs:comment>
        <rdfs:isDefinedBy rdf:resource="https://github.com/EmrahGuder/Renarration/#"/>
    </owl:Class>	
	
    <owl:Class rdf:about="&rn;TextSelector">
        <rdfs:label xml:lang="en">TextSelector</rdfs:label>
        <rdfs:comment xml:lang="en">
			subClass of rn:DocumentSelector and superclass of rn:PrefixSuffixSelector and rn:ByteSelector. The class describes a range of text either by the use of start and end positions or by using prefix and suffixes.
		</rdfs:comment>
        <rdfs:isDefinedBy rdf:resource="https://github.com/EmrahGuder/Renarration/#"/>
		<rdfs:subClassOf rdf:resource="&rn;DocumentSelector"/>
    </owl:Class>

    <owl:Class rdf:about="&rn;PrefixSuffixSelector">
        <rdfs:label xml:lang="en">PrefixSuffixSelector</rdfs:label>
        <rdfs:comment xml:lang="en">
			subClass of rn:TextSelector. The class describes a range of text by the use of prefix and suffix.
		</rdfs:comment>
        <rdfs:isDefinedBy rdf:resource="https://github.com/EmrahGuder/Renarration/#"/>
		<rdfs:subClassOf rdf:resource="&rn;TextSelector"/>
    </owl:Class>	
	
    <owl:Class rdf:about="&rn;ByteSelector">
        <rdfs:label xml:lang="en">ByteSelector</rdfs:label>
        <rdfs:comment xml:lang="en">
			subClass of rn:TextSelector. The class describes a range of text by the use of start and end bytes.
		</rdfs:comment>
        <rdfs:isDefinedBy rdf:resource="https://github.com/EmrahGuder/Renarration/#"/>
		<rdfs:subClassOf rdf:resource="&rn;TextSelector"/>
    </owl:Class>	
	
    <owl:Class rdf:about="&rn;BetweenSelector">
        <rdfs:label xml:lang="en">BetweenSelector</rdfs:label>
        <rdfs:comment xml:lang="en">
			subClass of rn:DocumentSelector. The class describes a selection between selection of two selectors.
		</rdfs:comment>
        <rdfs:isDefinedBy rdf:resource="https://github.com/EmrahGuder/Renarration/#"/>
		<rdfs:subClassOf rdf:resource="&rn;DocumentSelector"/>
    </owl:Class>	

    <owl:Class rdf:about="&rn;XPathSelector">
        <rdfs:label xml:lang="en">XPathSelector</rdfs:label>
        <rdfs:comment xml:lang="en">
			subClass of rn:DocumentSelector. The class describes a targeted segment by using a fragment identifier using xpath.
		</rdfs:comment>
        <rdfs:isDefinedBy rdf:resource="https://github.com/EmrahGuder/Renarration/#"/>
		<rdfs:subClassOf rdf:resource="&rn;DocumentSelector"/>
    </owl:Class>	
	
    <owl:Class rdf:about="&rn;MediaSelector">
        <rdfs:label xml:lang="en">MediaSelector</rdfs:label>
        <rdfs:comment xml:lang="en">
			subClass of rn:DocumentSelector. The class describes a targeted segment of any media on the Web by use of a fragment identifier.
		</rdfs:comment>
        <rdfs:isDefinedBy rdf:resource="https://github.com/EmrahGuder/Renarration/#"/>
		<rdfs:subClassOf rdf:resource="&rn;DocumentSelector"/>
    </owl:Class>	
	
    <owl:Class rdf:about="&rn;EmptySelector">
        <rdfs:label xml:lang="en">EmptySelector</rdfs:label>
        <rdfs:comment xml:lang="en">
			subClass of rn:DocumentSelector. The class describes no selection. Special class designed to be used with rn:BetweenSelector.
		</rdfs:comment>
        <rdfs:isDefinedBy rdf:resource="https://github.com/EmrahGuder/Renarration/#"/>
		<rdfs:subClassOf rdf:resource="&rn;DocumentSelector"/>
    </owl:Class>	
	
    <owl:Class rdf:about="&rn;Motivation">
        <rdfs:label xml:lang="en">Motivation</rdfs:label>
        <rdfs:comment xml:lang="en">
			subClass of skos:Concept. The reason behind the creation of a renarration or a renarration transformation. Motivations can be things like translation, simplification, correction, or alternative.
		</rdfs:comment>
        <rdfs:isDefinedBy rdf:resource="https://github.com/EmrahGuder/Renarration/#"/>
		<rdfs:subClassOf rdf:resource="&skos;Concept"/>
    </owl:Class>	
	
    <owl:Class rdf:about="&rn;List">
        <rdfs:label xml:lang="en">List</rdfs:label>
        <rdfs:comment xml:lang="en">
			subClass of rdf:Bag. Defines a list of narrations, which should be interpreted in defined order, for a source document or part of a source document.
		</rdfs:comment>
        <rdfs:isDefinedBy rdf:resource="https://github.com/EmrahGuder/Renarration/#"/>
		<rdfs:subClassOf rdf:resource="&rdf;Bag"/>
    </owl:Class>	
	
	<!-- Classes -->
	
	<!-- Named Individuals -->
	
    <owl:NamedIndividual rdf:about="&rn;actionScheme">
        <rdf:type rdf:resource="&skos;ConceptScheme"/>
        <rdfs:label xml:lang="en">actionScheme</rdfs:label>
        <rdfs:comment xml:lang="en">
			Instance of skos:ConceptScheme. The concept scheme for defining a set of instances of rn:Action.
		</rdfs:comment>
    </owl:NamedIndividual>
	
    <owl:NamedIndividual rdf:about="&rn;replace">
        <rdf:type rdf:resource="&rn;Action"/>
        <rdfs:comment xml:lang="en">
			Instance of rn:Action. The action that represents replacing content in a source document with new content which will reside in a target document.
		</rdfs:comment>
        <skos:prefLabel xml:lang="en">replace</skos:prefLabel>
        <skos:inScheme rdf:resource="&rn;actionScheme"/>
    </owl:NamedIndividual>	
	
    <owl:NamedIndividual rdf:about="&rn;remove">
        <rdf:type rdf:resource="&rn;Action"/>
        <rdfs:comment xml:lang="en">
			Instance of rn:Action. The action that represents replacing content in a source document with nothing in a target document.
		</rdfs:comment>
        <skos:prefLabel xml:lang="en">remove</skos:prefLabel>
        <skos:inScheme rdf:resource="&rn;actionScheme"/>
    </owl:NamedIndividual>	

	<owl:NamedIndividual rdf:about="&rn;insert">
        <rdf:type rdf:resource="&rn;Action"/>
        <rdfs:comment xml:lang="en">
			Instance of rn:Action. The action that represents insertion of content to a specified position in target document.
		</rdfs:comment>
        <skos:prefLabel xml:lang="en">insert</skos:prefLabel>
        <skos:inScheme rdf:resource="&rn;actionScheme"/>
    </owl:NamedIndividual>	
	
    <owl:NamedIndividual rdf:about="&rn;motivationScheme">
        <rdf:type rdf:resource="&skos;ConceptScheme"/>
        <rdfs:label xml:lang="en">motivationScheme</rdfs:label>
        <rdfs:comment xml:lang="en">
			The concept scheme for motivations.
		</rdfs:comment>
    </owl:NamedIndividual>	
	
	<owl:NamedIndividual rdf:about="&rn;translation">
        <rdf:type rdf:resource="&rn;Motivation"/>
        <rdfs:comment xml:lang="en">
			The motivation that represents interpretation of source content in another language.
		</rdfs:comment>
        <skos:prefLabel xml:lang="en">translation</skos:prefLabel>
        <skos:inScheme rdf:resource="&rn;motivationScheme"/>
    </owl:NamedIndividual>	

	<owl:NamedIndividual rdf:about="&rn;simplification">
        <rdf:type rdf:resource="&rn;Motivation"/>
        <rdfs:comment xml:lang="en">
			The motivation that represents simplifying content in a source document so that it will be easier to consume.
		</rdfs:comment>
        <skos:prefLabel xml:lang="en">simplification</skos:prefLabel>
        <skos:inScheme rdf:resource="&rn;motivationScheme"/>
    </owl:NamedIndividual>	

	<owl:NamedIndividual rdf:about="&rn;correction">
        <rdf:type rdf:resource="&rn;Motivation"/>
        <rdfs:comment xml:lang="en">
			The motivation that represents updating content either for verification or adjustment.
		</rdfs:comment>
        <skos:prefLabel xml:lang="en">correction</skos:prefLabel>
        <skos:inScheme rdf:resource="&rn;motivationScheme"/>
    </owl:NamedIndividual>	
	
	<owl:NamedIndividual rdf:about="&rn;alternative">
        <rdf:type rdf:resource="&rn;Motivation"/>
        <rdfs:comment xml:lang="en">
			The motivation that represents providing a new content which alternates content in a source document.
		</rdfs:comment>
        <skos:prefLabel xml:lang="en">alternative</skos:prefLabel>
        <skos:inScheme rdf:resource="&rn;motivationScheme"/>
    </owl:NamedIndividual>	
	
	<!-- Named Individuals -->
	
	
</rdf:RDF>